coq/theories/Utils/Rel.v
@@ -9,9 +9,6 @@ Definition relᵢ {I : Type} (A B : psh I) := forall i, A i -> B i -> Prop.
 #[global] Notation Transitiveᵢ R := (forall i, Transitive (R i)).
 #[global] Notation Subrelationᵢ R S := (forall i, subrelation (R i) (S i)).
 
-Definition flipᵢ {I : Type} {A B : psh I} (R : relᵢ A B) : relᵢ B A :=
-  fun i x y => R i y x.
-
 Print CompleteLattice.
 
 #[global] Program Instance CompleteLatticeRelᵢ {I : Type} {A B : psh I} : CompleteLattice (relᵢ A B) := {|
@@ -45,3 +42,6 @@ Definition seqᵢ {I} {X Y Z : psh I} (R0 : relᵢ X Y) (R1 : relᵢ Y Z) : rel�
 #[global] Notation "u ⨟⨟ v" := (ex_intro _ _ (conj u v)) (at level 70).
 
 Definition revᵢ {I} {X Y : psh I} (R : relᵢ X Y) : relᵢ Y X := fun i x y => R i y x.
+
+Definition orᵢ {I} {X Y : psh I} (R S : relᵢ X Y) : relᵢ X Y := fun i x y => R i x y \/ S i x y.
+#[global] Infix "∨ᵢ" := (orᵢ) (at level 70).
